aarch64 ainvs: bare minimum triage and sorrying
Starting point for AArch64 abstract invariant proofs.

In most cases, commented out or sorried what doesn't work. In some
cases, had to tweak definitions to get through. Marked all
problem/failure areas with FIXME AARCH64.

Signed-off-by: Rafal Kolanski <rafal.kolanski@proofcraft.systems>

proof/invariant-abstract/AARCH64/ArchVSpace_AI.thy
@@ -1,4 +1,5 @@
 (*
+ * Copyright 2022, Proofcraft Pty Ltd
  * Copyright 2020, Data61, CSIRO (ABN 41 687 119 230)
  *
  * SPDX-License-Identifier: GPL-2.0-only
@@ -12,11 +13,12 @@ theory ArchVSpace_AI
 imports VSpacePre_AI
 begin
 
-context Arch begin global_naming RISCV64
+context Arch begin global_naming AARCH64
 
+(* FIXME AARCH64
 definition kernel_mappings_only :: "(pt_index \<Rightarrow> pte) \<Rightarrow> 'z::state_ext state \<Rightarrow> bool" where
   "kernel_mappings_only pt s \<equiv>
-     has_kernel_mappings pt s \<and> (\<forall>idx. idx \<notin> kernel_mapping_slots \<longrightarrow> pt idx = InvalidPTE)"
+     has_kernel_mappings pt s \<and> (\<forall>idx. idx \<notin> kernel_mapping_slots \<longrightarrow> pt idx = InvalidPTE)" *)
 
 lemma find_vspace_for_asid_wp[wp]:
   "\<lbrace>\<lambda>s. (vspace_for_asid asid s = None \<longrightarrow> E InvalidRoot s) \<and>
@@ -34,7 +36,8 @@ lemma asid_word_bits [simp]: "asid_bits < word_bits"
 lemma vspace_at_asid_vs_lookup:
   "vspace_at_asid asid pt s \<Longrightarrow>
    vs_lookup_table max_pt_level asid 0 s = Some (max_pt_level, pt)"
-  by (simp add: vs_lookup_table_def vspace_at_asid_def vspace_for_asid_def in_omonad)
+  sorry (* FIXME AARCH64
+  by (simp add: vs_lookup_table_def vspace_at_asid_def vspace_for_asid_def in_omonad) *)
 
 lemma pt_at_asid_unique:
   "\<lbrakk> vspace_at_asid asid pt s; vspace_at_asid asid' pt s;
@@ -56,7 +59,7 @@ crunch valid_vs_lookup[wp]: do_machine_op "valid_vs_lookup"
 
 lemmas ackInterrupt_irq_masks = no_irq[OF no_irq_ackInterrupt]
 
-crunches sfence, hwASIDFlush, setVSpaceRoot
+crunches (* FIXME AARCH64 sfence, hwASIDFlush,*) setVSpaceRoot
   for underlying_memory_inv[wp]: "\<lambda>ms. P (underlying_memory ms)"
 
 
@@ -78,16 +81,17 @@ lemma asid_high_bits_of_or:
   apply (simp add: asid_high_bits_of_def word_size nth_ucast nth_shiftr asid_low_bits_def word_bits_def)
   done
 
+(* FIXME AARCH64
 lemma vs_lookup_clear_asid_table:
-  "vs_lookup_table bot_level asid vref (s\<lparr>arch_state := arch_state s \<lparr>riscv_asid_table :=
-                                            (riscv_asid_table (arch_state s)) (pptr := None)\<rparr>\<rparr>)
+  "vs_lookup_table bot_level asid vref (s\<lparr>arch_state := arch_state s \<lparr>arm_asid_table :=
+                                            (arm_asid_table (arch_state s)) (pptr := None)\<rparr>\<rparr>)
      = Some (level, p)
    \<Longrightarrow> vs_lookup_table bot_level asid vref s = Some (level, p)"
   by (fastforce simp: vs_lookup_table_def in_omonad pool_for_asid_def split: if_split_asm)
 
 lemma vs_lookup_target_clear_asid_table:
-  "vs_lookup_target bot_level asid vref (s\<lparr>arch_state := arch_state s \<lparr>riscv_asid_table :=
-                                            (riscv_asid_table (arch_state s)) (pptr := None)\<rparr>\<rparr>)
+  "vs_lookup_target bot_level asid vref (s\<lparr>arch_state := arch_state s \<lparr>arm_asid_table :=
+                                            (arm_asid_table (arch_state s)) (pptr := None)\<rparr>\<rparr>)
      = Some (level, p)
   \<Longrightarrow> vs_lookup_target bot_level asid vref s = Some (level, p)"
   apply (clarsimp simp: vs_lookup_target_def in_omonad vs_lookup_slot_def split: if_split_asm)
@@ -101,7 +105,7 @@ lemma vs_lookup_target_clear_asid_table:
 
 lemma valid_arch_state_unmap_strg:
   "valid_arch_state s \<longrightarrow>
-   valid_arch_state(s\<lparr>arch_state := arch_state s\<lparr>riscv_asid_table := (riscv_asid_table (arch_state s))(ptr := None)\<rparr>\<rparr>)"
+   valid_arch_state(s\<lparr>arch_state := arch_state s\<lparr>arm_asid_table := (arm_asid_table (arch_state s))(ptr := None)\<rparr>\<rparr>)"
   apply (clarsimp simp: valid_arch_state_def valid_asid_table_def)
   apply (rule conjI)
    apply (clarsimp simp add: ran_def)
@@ -112,7 +116,7 @@ lemma valid_arch_state_unmap_strg:
 
 lemma valid_vspace_objs_unmap_strg:
   "valid_vspace_objs s \<longrightarrow>
-   valid_vspace_objs(s\<lparr>arch_state := arch_state s\<lparr>riscv_asid_table := (riscv_asid_table (arch_state s))(ptr := None)\<rparr>\<rparr>)"
+   valid_vspace_objs(s\<lparr>arch_state := arch_state s\<lparr>arm_asid_table := (arm_asid_table (arch_state s))(ptr := None)\<rparr>\<rparr>)"
   apply (clarsimp simp: valid_vspace_objs_def)
   apply (blast dest: vs_lookup_clear_asid_table)
   done
@@ -120,40 +124,45 @@ lemma valid_vspace_objs_unmap_strg:
 
 lemma valid_vs_lookup_unmap_strg:
   "valid_vs_lookup s \<longrightarrow>
-   valid_vs_lookup(s\<lparr>arch_state := arch_state s\<lparr>riscv_asid_table := (riscv_asid_table (arch_state s))(ptr := None)\<rparr>\<rparr>)"
+   valid_vs_lookup(s\<lparr>arch_state := arch_state s\<lparr>arm_asid_table := (arm_asid_table (arch_state s))(ptr := None)\<rparr>\<rparr>)"
   apply (clarsimp simp: valid_vs_lookup_def)
   apply (blast dest: vs_lookup_target_clear_asid_table)
   done
+*)
 
 lemma asid_high_bits_shl:
   "is_aligned base asid_low_bits \<Longrightarrow> ucast (asid_high_bits_of base) << asid_low_bits = base"
   unfolding asid_high_bits_of_def asid_low_bits_def is_aligned_mask
   by word_eqI_solve
 
+(* FIXME AARCH64
 lemma valid_asid_map_unmap:
   "valid_asid_map s \<and> is_aligned base asid_low_bits \<longrightarrow>
-   valid_asid_map(s\<lparr>arch_state := arch_state s\<lparr>riscv_asid_table := (riscv_asid_table (arch_state s))(asid_high_bits_of base := None)\<rparr>\<rparr>)"
-  by (clarsimp simp: valid_asid_map_def)
+   valid_asid_map(s\<lparr>arch_state := arch_state s\<lparr>arm_asid_table := (arm_asid_table (arch_state s))(asid_high_bits_of base := None)\<rparr>\<rparr>)"
+  by (clarsimp simp: valid_asid_map_def) *)
 
 lemma asid_low_bits_word_bits:
   "asid_low_bits < word_bits"
   by (simp add: asid_low_bits_def word_bits_def)
 
+(* FIXME AARCH64
 lemma valid_vs_lookup_arch_update:
-  "riscv_asid_table (f (arch_state s)) = riscv_asid_table (arch_state s) \<and>
+  "arm_asid_table (f (arch_state s)) = arm_asid_table (arch_state s) \<and>
    riscv_kernel_vspace (f (arch_state s)) = riscv_kernel_vspace (arch_state s)
      \<Longrightarrow> valid_vs_lookup (arch_state_update f s) = valid_vs_lookup s"
-  by (simp add: valid_vs_lookup_def)
+  by (simp add: valid_vs_lookup_def) *)
 
 definition valid_unmap :: "vmpage_size \<Rightarrow> asid * vspace_ref \<Rightarrow> bool" where
   "valid_unmap sz \<equiv> \<lambda>(asid, vptr). 0 < asid \<and> is_aligned vptr (pageBitsForSize sz)"
 
+(* FIXME AARCH64 typechecks, might not make sense *)
 definition
-  "parent_for_refs \<equiv> \<lambda>(_, slot) cap.
-     \<exists>m. cap = ArchObjectCap (PageTableCap (table_base slot) m) \<and> m \<noteq> None"
+  "parent_for_refs \<equiv> \<lambda>(_, slot, pt_t) cap.
+     \<exists>pt_t m. cap = ArchObjectCap (PageTableCap (table_base pt_t slot) pt_t m) \<and> m \<noteq> None"
 
+(* FIXME AARCH64 typechecks, might not make sense *)
 definition
-  "same_ref \<equiv> \<lambda>(pte, slot) cap s.
+  "same_ref \<equiv> \<lambda>(pte, slot, pt_t) cap s.
      ((\<exists>p. pte_ref pte = Some p \<and> obj_refs cap = {p}) \<or> pte = InvalidPTE) \<and>
      (\<exists>level asid vref. vs_cap_ref cap = Some (asid, vref_for_level vref level) \<and>
                         vs_lookup_slot level asid vref s = Some (level, slot) \<and>
@@ -166,7 +175,7 @@ definition
       and (cte_wp_at (\<lambda>c. vs_cap_ref c = None) ptr or (\<lambda>s. cte_wp_at (\<lambda>c. same_ref m c s) ptr s))
       and cte_wp_at is_frame_cap ptr
       and same_ref m (ArchObjectCap acap)
-      and valid_slots m
+      \<comment> \<open>(* FIXME AARCH64 and valid_slots m \<close>
       and valid_arch_cap acap
       and K (is_PagePTE (fst m) \<or> fst m = InvalidPTE)
       and (\<lambda>s. \<exists>slot. cte_wp_at (parent_for_refs m) slot s)
@@ -178,20 +187,21 @@ definition
             valid_arch_cap acap s
   | PageGetAddr ptr \<Rightarrow> \<top>"
 
+(* FIXME AARCH64 typechecks, needs fixing *)
 definition
   "valid_pti pti \<equiv> case pti of
-     PageTableMap acap cslot pte pt_slot \<Rightarrow>
-       pte_at pt_slot and K (wellformed_pte pte \<and> is_PageTablePTE pte) and
+     PageTableMap acap cslot pte pt_slot FIXME_level \<Rightarrow>
+       pte_at FIXME_level pt_slot and K (wellformed_pte pte \<and> is_PageTablePTE pte) and
        valid_arch_cap acap and
        cte_wp_at (\<lambda>c. is_arch_update (ArchObjectCap acap) c \<and> cap_asid c = None) cslot and
-       invalid_pte_at pt_slot and
+       \<comment> \<open>(* FIXME AARCH64 invalid_pte_at pt_slot and\<close>
        (\<lambda>s. \<exists>p' level asid vref.
                 vs_cap_ref_arch acap = Some (asid, vref_for_level vref level)
                 \<and> vs_lookup_slot level asid vref s = Some (level, pt_slot)
                 \<and> valid_pte level pte s
                 \<and> pte_ref pte = Some p' \<and> obj_refs (ArchObjectCap acap) = {p'}
                 \<and> (\<exists>ao. ko_at (ArchObj ao) p' s \<and> valid_vspace_obj (level-1) ao s)
-                \<and> pts_of s p' = Some empty_pt
+                \<and> pts_of s p' = Some (empty_pt FIXME_level)
                 \<and> vref \<in> user_region) and
        K (is_PageTableCap acap \<and> cap_asid_arch acap \<noteq> None)
    | PageTableUnmap acap cslot \<Rightarrow>
@@ -206,16 +216,17 @@ definition
 crunches unmap_page
   for aligned [wp]: pspace_aligned
   and "distinct" [wp]: pspace_distinct
-  and valid_objs[wp]: valid_objs
+  (* FIXME AARCH64: and valid_objs[wp]: valid_objs *)
   and caps_of_state[wp]: "\<lambda>s. P (caps_of_state s)"
   (wp: crunch_wps simp: crunch_simps)
 
+(* FIXME AARCH64:
 lemma set_cap_valid_slots[wp]:
   "set_cap cap p \<lbrace>valid_slots slots\<rbrace>"
   apply (cases slots, clarsimp simp: valid_slots_def)
   apply (wpsimp wp: hoare_vcg_ball_lift hoare_vcg_all_lift hoare_vcg_imp_lift')
   apply blast
-  done
+  done *)
 
 lemma pt_lookup_from_level_inv[wp]:
   "\<lbrace>Q and E\<rbrace> pt_lookup_from_level level pt_ptr vptr target_pt_ptr \<lbrace>\<lambda>_. Q\<rbrace>,\<lbrace>\<lambda>_. E\<rbrace>"
@@ -230,7 +241,7 @@ qed
 
 crunches unmap_page_table
   for aligned[wp]: pspace_aligned
-  and valid_objs[wp]: valid_objs
+  (* FIXME AARCH64: and valid_objs[wp]: valid_objs *)
   and "distinct"[wp]: pspace_distinct
   and caps_of_state[wp]: "\<lambda>s. P (caps_of_state s)"
   and typ_at[wp]: "\<lambda>s. P (typ_at T p s)"
@@ -273,11 +284,12 @@ lemma dmo_setVMRoot[wp]:
   apply (auto simp: setVSpaceRoot_def machine_op_lift_def machine_rest_lift_def in_monad select_f_def)
   done
 
+(* FIXME AARCH64: different machine ops here
 lemma dmo_sfence[wp]:
   "do_machine_op sfence \<lbrace>invs\<rbrace>"
   apply (wp dmo_invs)
   apply (auto simp: sfence_def machine_op_lift_def machine_rest_lift_def in_monad select_f_def)
-  done
+  done *)
 
 lemma find_vspace_for_asid_inv[wp]:
   "\<lbrace>P and Q\<rbrace> find_vspace_for_asid asid \<lbrace>\<lambda>_. P\<rbrace>, \<lbrace>\<lambda>_. Q\<rbrace>"
@@ -286,12 +298,14 @@ lemma find_vspace_for_asid_inv[wp]:
 lemma set_vm_root_typ_at[wp]:
   "set_vm_root t \<lbrace>\<lambda>s. P (typ_at T p s)\<rbrace>"
   unfolding set_vm_root_def
-  by (wpsimp simp: if_distribR wp: get_cap_wp)
+  sorry (* FIXME AARCH64
+  by (wpsimp simp: if_distribR wp: get_cap_wp) *)
 
 lemma set_vm_root_invs[wp]:
   "set_vm_root t \<lbrace>invs\<rbrace>"
   unfolding set_vm_root_def
-  by (wpsimp simp: if_distribR wp: get_cap_wp)
+  sorry (* FIXME AARCH64
+  by (wpsimp simp: if_distribR wp: get_cap_wp) *)
 
 crunch pred_tcb_at[wp]: set_vm_root "pred_tcb_at proj P t"
   (simp: crunch_simps)
@@ -320,13 +334,14 @@ lemma set_cap_valid_pte_stronger:
 
 (* FIXME: move *)
 lemma valid_cap_to_pt_cap:
-  "\<lbrakk>valid_cap c s; obj_refs c = {p}; pt_at p s\<rbrakk> \<Longrightarrow> is_pt_cap c"
+  "\<lbrakk>valid_cap c s; obj_refs c = {p}; pt_at pt_t p s\<rbrakk> \<Longrightarrow> is_pt_cap c"
   by (clarsimp simp: valid_cap_def obj_at_def is_obj_defs is_pt_cap_def valid_arch_cap_ref_def
               split: cap.splits option.splits arch_cap.splits if_splits)
 
+(* FIXME AARCH64:
 lemma set_cap_invalid_pte[wp]:
   "set_cap cap p' \<lbrace>invalid_pte_at p\<rbrace>"
-  unfolding invalid_pte_at_def by wpsimp
+  unfolding invalid_pte_at_def by wpsimp *)
 
 lemma valid_cap_obj_ref_pt:
   "\<lbrakk> s \<turnstile> cap; s \<turnstile> cap'; obj_refs cap = obj_refs cap' \<rbrakk>
@@ -359,7 +374,7 @@ lemmas store_pte_cte_wp_at1[wp]
     = hoare_cte_wp_caps_of_state_lift [OF store_pte_caps_of_state]
 
 lemma mdb_cte_at_store_pte[wp]:
-  "store_pte y pte \<lbrace>\<lambda>s. mdb_cte_at (swp (cte_wp_at ((\<noteq>) cap.NullCap)) s) (cdt s)\<rbrace>"
+  "store_pte pt_t y pte \<lbrace>\<lambda>s. mdb_cte_at (swp (cte_wp_at ((\<noteq>) cap.NullCap)) s) (cdt s)\<rbrace>"
   apply (clarsimp simp:mdb_cte_at_def)
   apply (simp only: imp_conv_disj)
   apply (wpsimp wp: hoare_vcg_disj_lift hoare_vcg_all_lift simp: store_pte_def set_pt_def)
@@ -410,6 +425,7 @@ lemma arch_update_cap_invs_map:
    apply (clarsimp simp: is_valid_vtable_root_def vs_cap_ref_def vs_cap_ref_arch_def split: cap.splits)
    apply (simp split: arch_cap.splits option.splits;
           clarsimp simp: cap_master_cap_simps vs_cap_ref_arch_def)
+  sorry (* FIXME AARCH64
   apply (rule conjI)
    apply (rule ext)
    apply (simp add: cap_master_cap_def split: cap.splits arch_cap.splits)
@@ -464,7 +480,7 @@ lemma arch_update_cap_invs_map:
                  elim!: ranE cong: master_cap_eq_is_device_cap_eq
              | rule conjI)+
   apply (clarsimp dest!: master_cap_eq_is_device_cap_eq)
-  done
+  done *)
 
 lemma pool_for_asid_ap_at:
   "\<lbrakk> pool_for_asid asid s = Some p; valid_arch_state s \<rbrakk> \<Longrightarrow> asid_pool_at p s"
@@ -517,7 +533,7 @@ lemma arch_update_cap_invs_unmap_page:
   done
 
 lemma mask_cap_PageTableCap[simp]:
-  "mask_cap R (ArchObjectCap (PageTableCap p data)) = ArchObjectCap (PageTableCap p data)"
+  "mask_cap R (ArchObjectCap (PageTableCap p pt_t data)) = ArchObjectCap (PageTableCap p pt_t data)"
   by (clarsimp simp: mask_cap_def cap_rights_update_def acap_rights_update_def)
 
 lemma arch_update_cap_pspace':
@@ -541,7 +557,7 @@ lemma arch_update_cap_invs_unmap_page_table:
              and real_cte_at p
              and invs and valid_cap cap
              and (\<lambda>s. cte_wp_at (\<lambda>c. is_final_cap' c s) p s)
-             and (\<lambda>s. pts_of s (obj_ref_of cap) = Some empty_pt)
+             and (\<lambda>s. pts_of s (obj_ref_of cap) = Some (empty_pt FIXME_level))
              and (\<lambda>s. cte_wp_at (\<lambda>c. \<forall>asid vref level. vs_cap_ref c = Some (asid, vref)
                                 \<longrightarrow> vs_lookup_target level asid vref s \<noteq> Some (level, obj_ref_of cap)) p s)
              and K (is_pt_cap cap \<and> vs_cap_ref cap = None)\<rbrace>
@@ -579,18 +595,20 @@ lemma arch_update_cap_invs_unmap_page_table:
                           cte_wp_at_caps_of_state)
     apply fastforce
    apply (clarsimp simp: obj_at_def empty_table_def in_omonad)
+  sorry (* FIXME AARCH64
   apply fastforce
-  done
+  done *)
 
+(* FIXME AARCH64
 lemma global_refs_arch_update_eq:
   "riscv_global_pts (f (arch_state s)) = riscv_global_pts (arch_state s) \<Longrightarrow>
    global_refs (arch_state_update f s) = global_refs s"
-  by (simp add: global_refs_def)
+  by (simp add: global_refs_def) *)
 
 lemma not_in_global_refs_vs_lookup:
   "(\<exists>\<rhd> (level,p)) s \<and> valid_vs_lookup s \<and> valid_global_refs s
             \<and> valid_arch_state s \<and> valid_global_objs s
-            \<and> pt_at p s
+            \<and> pt_at pt_t p s
         \<longrightarrow> p \<notin> global_refs s"
   apply clarsimp
   apply (cases "level = asid_pool_level"; simp)
@@ -603,9 +621,11 @@ lemma not_in_global_refs_vs_lookup:
   apply (simp add: cap_range_def)
   done
 
+(* FIXME AARCH64: different machine ops here
 lemma no_irq_sfence[wp,intro!]: "no_irq sfence"
-  by (wpsimp simp: sfence_def no_irq_def machine_op_lift_def machine_rest_lift_def)
+  by (wpsimp simp: sfence_def no_irq_def machine_op_lift_def machine_rest_lift_def) *)
 
+(* FIXME AARCH64
 lemma pt_lookup_from_level_wp:
   "\<lbrace>\<lambda>s. (\<forall>level pt' pte.
             pt_walk top_level level top_level_pt vref (ptes_of s) = Some (level, pt') \<longrightarrow>
@@ -652,12 +672,13 @@ next
     apply (subst (asm) bit0.leq_minus1_less[symmetric], assumption)
     apply simp
     done
-qed
+qed *)
 
 (* weaker than pspace_aligned_pts_ofD, but still sometimes useful because it matches better *)
 lemma pts_of_Some_alignedD:
-  "\<lbrakk> pts_of s p = Some pt; pspace_aligned s \<rbrakk> \<Longrightarrow> is_aligned p pt_bits"
-  by (drule pspace_aligned_pts_ofD; simp)
+  "\<lbrakk> pts_of s p = Some pt; pspace_aligned s \<rbrakk> \<Longrightarrow> is_aligned p (pt_bits pt_t)"
+  sorry (* FIXME AARCH64: might not make sense
+  by (drule pspace_aligned_pts_ofD; simp) *)
 
 lemma vs_lookup_target_not_global:
   "\<lbrakk> vs_lookup_target level asid vref s = Some (level, pt); vref \<in> user_region; invs s \<rbrakk>
@@ -686,6 +707,7 @@ lemma unmap_page_table_invs[wp]:
    apply (wp dmo_invs | wpc | simp)+
      apply (rule_tac Q="\<lambda>_. invs" in hoare_post_imp)
       apply safe
+  sorry (* FIXME AARCH64
        apply (drule_tac Q="\<lambda>_ m'. underlying_memory m' p =
                                   underlying_memory m p" in use_valid)
          apply ((wp | simp)+)[3]
@@ -707,7 +729,7 @@ lemma unmap_page_table_invs[wp]:
    apply (simp add: table_index_max_level_slots)
   apply (drule (1) vs_lookup_table_target)
   apply (drule vs_lookup_target_not_global, erule vref_for_level_user_region; simp)
-  done
+  done *)
 
 lemma final_cap_lift:
   assumes x: "\<And>P. \<lbrace>\<lambda>s. P (caps_of_state s)\<rbrace> f \<lbrace>\<lambda>rv s. P (caps_of_state s)\<rbrace>"
@@ -719,41 +741,45 @@ lemmas store_pte_final_cap[wp] = final_cap_lift [OF store_pte_caps_of_state]
 lemmas unmap_page_table_final_cap[wp] = final_cap_lift [OF unmap_page_table_caps_of_state]
 
 lemma store_pte_vspace_for_asid[wp]:
-  "store_pte p pte \<lbrace>\<lambda>s. P (vspace_for_asid asid s)\<rbrace>"
-  by (wp vspace_for_asid_lift)
+  "store_pte pte_t p pte \<lbrace>\<lambda>s. P (vspace_for_asid asid s)\<rbrace>"
+  sorry (* FIXME AARCH64
+  by (wp vspace_for_asid_lift) *)
 
 lemma mapM_swp_store_pte_invs_unmap:
   "\<lbrace>invs and
-    (\<lambda>s. \<forall>sl\<in>set slots. table_base sl \<notin> global_refs s \<and>
-                        (\<forall>asid. vspace_for_asid asid s \<noteq> Some (table_base sl))) and
+    (\<lambda>s. \<forall>sl\<in>set slots. table_base pt_t sl \<notin> global_refs s \<and>
+                        (\<forall>asid. vspace_for_asid asid s \<noteq> Some (table_base pt_t sl))) and
     K (pte = InvalidPTE)\<rbrace>
-  mapM (swp store_pte pte) slots \<lbrace>\<lambda>_. invs\<rbrace>"
+  mapM (swp (store_pte pte_t) pte) slots \<lbrace>\<lambda>_. invs\<rbrace>"
   apply (rule hoare_post_imp)
    prefer 2
    apply (rule mapM_wp')
    apply simp
+   sorry (* FIXME AARCH64 check lemma statement
    apply (wp store_pte_invs hoare_vcg_const_Ball_lift hoare_vcg_ex_lift hoare_vcg_all_lift)
    apply (clarsimp simp: wellformed_pte_def)
   apply simp
-  done
+  done *)
 
 lemma mapM_x_swp_store_pte_invs_unmap:
-  "\<lbrace>invs and (\<lambda>s. \<forall>sl \<in> set slots. table_base sl \<notin> global_refs s \<and>
-                                    (\<forall>asid. vspace_for_asid asid s \<noteq> Some (table_base sl))) and
+  "\<lbrace>invs and (\<lambda>s. \<forall>sl \<in> set slots. table_base pt_t sl \<notin> global_refs s \<and>
+                                    (\<forall>asid. vspace_for_asid asid s \<noteq> Some (table_base pt_t sl))) and
     K (pte = InvalidPTE)\<rbrace>
-  mapM_x (swp store_pte pte) slots \<lbrace>\<lambda>_. invs\<rbrace>"
-  by (simp add: mapM_x_mapM | wp mapM_swp_store_pte_invs_unmap)+
+  mapM_x (swp (store_pte pte_t) pte) slots \<lbrace>\<lambda>_. invs\<rbrace>"
+  sorry (* FIXME AARCH64 check lemma statement
+  by (simp add: mapM_x_mapM | wp mapM_swp_store_pte_invs_unmap)+ *)
 
 lemma vs_lookup_table_step:
   "\<lbrakk> vs_lookup_table level asid vref s = Some (level, pt'); level \<le> max_pt_level; 0 < level;
-     ptes_of s (pt_slot_offset level pt' vref) = Some pte; is_PageTablePTE pte;
+     ptes_of s pt_t  (pt_slot_offset level pt' vref) = Some pte; is_PageTablePTE pte;
      pte_ref pte = Some pt \<rbrakk> \<Longrightarrow>
     vs_lookup_table (level-1) asid vref s = Some (level-1, pt)"
   apply (subst vs_lookup_split_Some[where level'=level]; assumption?)
    apply (simp add: order_less_imp_le)
   apply (subst pt_walk.simps)
   apply (clarsimp simp: in_omonad is_PageTablePTE_def pptr_from_pte_def)
-  done
+  sorry (* FIXME AARCH64
+  done *)
 
 lemma pte_ref_Some_cases:
   "(pte_ref pte = Some ref) = ((is_PageTablePTE pte \<or> is_PagePTE pte) \<and> ref = pptr_from_pte pte)"
@@ -761,15 +787,16 @@ lemma pte_ref_Some_cases:
 
 lemma max_pt_level_eq_minus_one:
   "level - 1 = max_pt_level \<Longrightarrow> level = asid_pool_level"
-  unfolding level_defs by auto
+  sorry (* FIXME AARCH64
+  unfolding level_defs by auto *)
 
 lemma store_pte_invalid_vs_lookup_target_unmap:
   "\<lbrace>\<lambda>s. (\<exists>level'. vs_lookup_slot level' asid vref s = Some (level', p) \<and>
-                  pte_refs_of s p = Some p') \<and>
+                  pte_refs_of pt_t p s = Some p') \<and>
          vref \<in> user_region \<and>
          pspace_aligned s \<and> valid_asid_table s \<and> valid_vspace_objs s \<and>
          unique_table_refs s \<and> valid_vs_lookup s \<and> valid_caps (caps_of_state s) s \<rbrace>
-   store_pte p InvalidPTE
+   store_pte pt_t p InvalidPTE
    \<lbrace>\<lambda>_ s. vs_lookup_target level asid vref s \<noteq> Some (level, p')\<rbrace>"
   unfolding store_pte_def set_pt_def
   supply fun_upd_apply[simp del]
@@ -780,6 +807,7 @@ lemma store_pte_invalid_vs_lookup_target_unmap:
    apply (clarsimp simp: obj_at_def in_omonad)
    apply (frule_tac p=p in pspace_alignedD, assumption)
    apply (simp add: bit_simps)
+  sorry (* FIXME AARCH64
   apply (frule (5) valid_vspace_objs_strong_slotD)
   apply (clarsimp simp: vs_lookup_slot_def split: if_split_asm)
   apply (clarsimp simp: in_omonad pte_ref_Some_cases)
@@ -854,20 +882,21 @@ lemma store_pte_invalid_vs_lookup_target_unmap:
   apply (clarsimp simp: in_omonad)
   apply (subst (asm) (3) pte_of_def)
   apply (clarsimp simp: in_omonad fun_upd_apply split: if_split_asm)
-  done
+  done *)
 
 lemma pt_lookup_from_level_wrp:
   "\<lbrace>\<lambda>s. \<exists>asid. vspace_for_asid asid s = Some top_level_pt \<and>
                (\<forall>level slot pte.
                    vs_lookup_slot level asid vref s = Some (level, slot) \<longrightarrow>
-                   ptes_of s slot = Some pte \<longrightarrow>
+                   ptes_of s pt_t slot = Some pte \<longrightarrow>
                    is_PageTablePTE pte \<longrightarrow>
                    pte_ref pte = Some pt \<longrightarrow>
-                   Q slot s) \<and>
+                   Q (slot, FIXME_level) s) \<and>
                ((\<forall>level<max_pt_level. vs_lookup_table level asid vref s \<noteq> Some (level, pt)) \<longrightarrow>
                    E InvalidRoot s)\<rbrace>
    pt_lookup_from_level max_pt_level top_level_pt vref pt
    \<lbrace>Q\<rbrace>, \<lbrace>E\<rbrace>"
+  sorry (* FIXME AARCH64 check lemma statement
   apply (wp pt_lookup_from_level_wp)
   apply (clarsimp simp: vspace_for_asid_def)
   apply (rule conjI; clarsimp)
@@ -879,10 +908,10 @@ lemma pt_lookup_from_level_wrp:
    apply simp
   apply (erule allE, erule (1) impE)
   apply (clarsimp simp: vs_lookup_table_def split: if_split_asm)
-  done
+  done *)
 
 lemma unmap_page_table_not_target:
-  "\<lbrace>\<lambda>s. pt_at pt s \<and> pspace_aligned s \<and> valid_asid_table s \<and> valid_vspace_objs s \<and>
+  "\<lbrace>\<lambda>s. pt_at pt_t pt s \<and> pspace_aligned s \<and> valid_asid_table s \<and> valid_vspace_objs s \<and>
         unique_table_refs s \<and> valid_vs_lookup s \<and> valid_caps (caps_of_state s) s \<and>
         0 < asid \<and> vref \<in> user_region \<and> vspace_for_asid asid s \<noteq> Some pt \<and>
         asid' = asid \<and> pt' = pt \<and> vref' = vref \<rbrace>
@@ -890,6 +919,7 @@ lemma unmap_page_table_not_target:
    \<lbrace>\<lambda>_ s. vs_lookup_target level asid' vref' s \<noteq> Some (level, pt')\<rbrace>"
   unfolding unmap_page_table_def
   apply (wpsimp wp: store_pte_invalid_vs_lookup_target_unmap pt_lookup_from_level_wrp)
+  sorry (* FIXME AARCH64
   apply (rule conjI; clarsimp)
    apply (clarsimp simp: vs_lookup_target_def vs_lookup_slot_def vs_lookup_table_def
                    split: if_split_asm;
@@ -912,7 +942,7 @@ lemma unmap_page_table_not_target:
   apply (drule (4) vs_lookup_table_step, simp)
   apply (prop_tac "level - 1 < max_pt_level", erule (1) bit0.minus_one_leq_less)
   apply fastforce
-  done
+  done *)
 
 lemma is_final_cap_caps_of_state_2D:
   "\<lbrakk> caps_of_state s p = Some cap; caps_of_state s p' = Some cap';
@@ -928,36 +958,39 @@ lemma is_final_cap_caps_of_state_2D:
                         prod_eqI)
   done
 
-crunch underlying_memory[wp]: ackInterrupt, hwASIDFlush, read_stval, setVSpaceRoot, sfence
+crunch underlying_memory[wp]: ackInterrupt, setVSpaceRoot (*, FIXME AARCH64 hwASIDFlush, read_stval, sfence*)
   "\<lambda>m'. underlying_memory m' p = um"
   (simp: cache_machine_op_defs machine_op_lift_def machine_rest_lift_def split_def)
 
-crunches storeWord, ackInterrupt, hwASIDFlush, read_stval, setVSpaceRoot, sfence
+crunches storeWord, ackInterrupt, setVSpaceRoot (*, hwASIDFlush, read_stval, sfence *)
   for device_state_inv[wp]: "\<lambda>ms. P (device_state ms)"
   (simp: crunch_simps)
 
+(* FIXME AARCH64
 crunch pspace_respects_device_region[wp]: perform_page_invocation "pspace_respects_device_region"
   (simp: crunch_simps wp: crunch_wps set_object_pspace_respects_device_region
          pspace_respects_device_region_dmo)
+*)
 
 lemma mapM_x_store_pte_caps_of_state[wp]:
-  "mapM_x (swp store_pte InvalidPTE) slots \<lbrace>\<lambda>s. P (caps_of_state s)\<rbrace>"
+  "mapM_x (swp (store_pte pt_t) InvalidPTE) slots \<lbrace>\<lambda>s. P (caps_of_state s)\<rbrace>"
   by (wpsimp wp: mapM_x_wp')
 
 lemma mapM_x_store_pte_valid_cap[wp]:
-  "mapM_x (swp store_pte InvalidPTE) slots \<lbrace>valid_cap cap\<rbrace>"
+  "mapM_x (swp (store_pte pt_t) InvalidPTE) slots \<lbrace>valid_cap cap\<rbrace>"
   by (wpsimp wp: mapM_x_wp')
 
 lemma mapM_x_store_pte_final_cap[wp]:
-  "mapM_x (swp store_pte InvalidPTE) slots \<lbrace>is_final_cap' cap\<rbrace>"
+  "mapM_x (swp (store_pte pt_t) InvalidPTE) slots \<lbrace>is_final_cap' cap\<rbrace>"
   by (wpsimp wp: final_cap_lift)
 
 lemma mapM_x_store_pte_empty[wp]:
-  "\<lbrace> \<lambda>s. slots = [p , p + (1 << pte_bits) .e. p + (1 << pt_bits) - 1] \<and>
-         is_aligned p pt_bits \<and> pt_at p s \<rbrace>
-   mapM_x (swp store_pte InvalidPTE) slots
-   \<lbrace> \<lambda>_ s. pts_of s p = Some empty_pt \<rbrace>"
+  "\<lbrace> \<lambda>s. slots = [p , p + (1 << pte_bits) .e. p + (1 << pt_bits pt_t) - 1] \<and>
+         is_aligned p (pt_bits pt_t) \<and> pt_at pt_t p s \<rbrace>
+   mapM_x (swp (store_pte pt_t) InvalidPTE) slots
+   \<lbrace> \<lambda>_ s. pts_of s p = Some (empty_pt pt_t) \<rbrace>"
   apply wp_pre
+  sorry (* FIXME AARCH64
    apply (rule_tac I="\<lambda>s. slots = [p , p + (1 << pte_bits) .e. p + (1 << pt_bits) - 1] \<and>
                           is_aligned p pt_bits \<and> pt_at p s" and
                    V="\<lambda>xs s. \<forall>p' \<in> set slots - set xs. ptes_of s p' = Some InvalidPTE"
@@ -980,19 +1013,21 @@ lemma mapM_x_store_pte_empty[wp]:
     apply (fastforce simp: table_index_plus_ucast table_base_plus_ucast)
    apply (wpsimp wp: store_pte_ptes_of)
   apply simp
-  done
+  done *)
 
 lemma vs_lookup_slot_pool_for_asid:
   "(vs_lookup_slot asid_pool_level asid vref s = Some (level, slot)) =
    (pool_for_asid asid s = Some slot \<and> level = asid_pool_level)"
   by (auto simp: vs_lookup_slot_def vs_lookup_table_def in_omonad)
 
+(* FIXME AARCH64
 lemma ptes_of_upd:
   "\<lbrakk> pts (table_base p) = Some pt; is_aligned p pte_bits \<rbrakk> \<Longrightarrow>
    (\<lambda>p'. pte_of p' (pts(table_base p \<mapsto> pt(table_index p := pte)))) =
    ((\<lambda>p'. pte_of p' pts)(p \<mapsto> pte))"
-  by (rule ext) (auto simp: pte_of_def obind_def split: option.splits dest: pte_ptr_eq)
+  by (rule ext) (auto simp: pte_of_def obind_def split: option.splits dest: pte_ptr_eq) *)
 
+(* FIXME AARCH64 function update syntax doesn't work here, not obvious how to fix
 lemma pt_walk_upd_Invalid:
   "pt_walk top_level level pt_ptr vref (ptes(p \<mapsto> InvalidPTE)) = Some (level, p') \<Longrightarrow>
    pt_walk top_level level pt_ptr vref ptes = Some (level, p')"
@@ -1002,13 +1037,14 @@ lemma pt_walk_upd_Invalid:
   apply (erule disjE; clarsimp)
   apply (subst pt_walk.simps)
   apply (clarsimp simp: in_omonad)
-  done
+  done *)
 
 lemma store_pte_unreachable:
-  "store_pte p InvalidPTE \<lbrace>\<lambda>s. vs_lookup_target level asid vref s \<noteq> Some (level, p')\<rbrace>"
+  "store_pte pt_t p InvalidPTE \<lbrace>\<lambda>s. vs_lookup_target level asid vref s \<noteq> Some (level, p')\<rbrace>"
   unfolding store_pte_def set_pt_def
   supply fun_upd_apply[simp del] vs_lookup_slot_pool_for_asid[simp]
   apply (wpsimp wp: set_object_wp simp: obj_at_def)
+  sorry (* FIXME AARCH64
   apply (prop_tac "asid_pools_of s (table_base p) = None", clarsimp simp: opt_map_def)
   apply (erule notE)
   apply (cases "level = asid_pool_level"; clarsimp simp: vs_lookup_target_def in_omonad)
@@ -1020,15 +1056,15 @@ lemma store_pte_unreachable:
   apply (clarsimp cong: conj_cong)
   apply (rule conjI, clarsimp)
   apply (clarsimp simp: ptes_of_def in_omonad fun_upd_apply split: if_split_asm)
-  done
+  done *)
 
 lemma mapM_x_store_pte_unreachable:
-  "mapM_x (swp store_pte InvalidPTE) slots
+  "mapM_x (swp (store_pte pt_t) InvalidPTE) slots
    \<lbrace>\<lambda>s. vs_lookup_target level asid vref s \<noteq> Some (level, p)\<rbrace>"
   by (wpsimp wp: mapM_x_wp' store_pte_unreachable)
 
 lemma mapM_x_typ_at[wp]:
-  "mapM_x (swp store_pte InvalidPTE) slots \<lbrace>\<lambda>s. P (typ_at T p s)\<rbrace>"
+  "mapM_x (swp (store_pte pt_t) InvalidPTE) slots \<lbrace>\<lambda>s. P (typ_at T p s)\<rbrace>"
   by (wpsimp wp: mapM_x_wp')
 
 crunches unmap_page_table
@@ -1039,7 +1075,8 @@ crunches unmap_page_table
 lemma vspace_for_asid_target:
   "vspace_for_asid asid s = Some pt \<Longrightarrow>
    vs_lookup_target asid_pool_level asid 0 s = Some (asid_pool_level, pt)"
-  by (clarsimp simp: vs_lookup_target_def vs_lookup_slot_pool_for_asid vspace_for_asid_def in_omonad)
+  sorry (* FIXME AARCH64
+  by (clarsimp simp: vs_lookup_target_def vs_lookup_slot_pool_for_asid vspace_for_asid_def in_omonad) *)
 
 lemma perform_pt_inv_unmap_invs[wp]:
   "\<lbrace>invs and valid_pti (PageTableUnmap cap ct_slot)\<rbrace> perform_pt_inv_unmap cap ct_slot \<lbrace>\<lambda>_. invs\<rbrace>"
@@ -1060,6 +1097,7 @@ lemma perform_pt_inv_unmap_invs[wp]:
   apply (clarsimp simp: wellformed_mapdata_def valid_cap_def cap_aligned_def cap_master_cap_simps)
   apply (rule conjI)
    apply clarsimp
+  sorry (* FIXME AARCH64
    apply (prop_tac "is_aligned p pt_bits", simp add: bit_simps)
    apply (subst (asm) upto_enum_step_shift_red; simp?)
      apply (simp add: bit_simps)
@@ -1083,21 +1121,22 @@ lemma perform_pt_inv_unmap_invs[wp]:
    apply (drule (1) unique_table_refsD[rotated]; clarsimp)
    apply (clarsimp simp: is_cap_simps)
   apply (fastforce intro: valid_objs_caps simp: bit_simps)
-  done
+  done *)
 
 lemma set_cap_vspace_for_asid[wp]:
   "set_cap p cap \<lbrace>\<lambda>s. P (vspace_for_asid asid s)\<rbrace>"
   by (wpsimp wp: vspace_for_asid_lift)
 
 lemma cap_asid_None_pt:
-  "(cap_asid (ArchObjectCap (PageTableCap p m)) = None) = (m = None)"
+  "(cap_asid (ArchObjectCap (PageTableCap p pt_t m)) = None) = (m = None)"
   by (cases m; clarsimp simp: cap_asid_def)
 
 lemma perform_pt_inv_map_invs[wp]:
-  "\<lbrace>invs and valid_pti (PageTableMap cap ct_slot pte slot)\<rbrace>
-   perform_pt_inv_map cap ct_slot pte slot
+  "\<lbrace>invs and valid_pti (PageTableMap cap ct_slot pte slot level)\<rbrace>
+   perform_pt_inv_map cap ct_slot pte slot level
    \<lbrace>\<lambda>_. invs\<rbrace>"
   unfolding perform_pt_inv_map_def
+  sorry (* FIXME AARCH64
   apply (wpsimp wp: store_pte_invs arch_update_cap_invs_map hoare_vcg_all_lift hoare_vcg_imp_lift')
   apply (clarsimp simp: valid_pti_def cte_wp_at_caps_of_state is_arch_update_def is_cap_simps
                         is_PageTableCap_def cap_master_cap_simps invalid_pte_at_def)
@@ -1163,11 +1202,12 @@ lemma perform_pt_inv_map_invs[wp]:
    apply (drule (1) unique_table_refsD[rotated]; clarsimp)
   apply (frule pt_slot_offset_vref_for_level; simp)
   apply (cases ct_slot, fastforce)
-  done
+  done *)
 
 lemma perform_page_table_invocation_invs[wp]:
   "\<lbrace>invs and valid_pti pti\<rbrace> perform_page_table_invocation pti \<lbrace>\<lambda>_. invs\<rbrace>"
-  unfolding perform_page_table_invocation_def by (cases pti; wpsimp)
+  sorry (* FIXME AARCH64
+  unfolding perform_page_table_invocation_def by (cases pti; wpsimp) *)
 
 crunch cte_wp_at [wp]: unmap_page "\<lambda>s. P (cte_wp_at P' p s)"
   (wp: crunch_wps simp: crunch_simps)
@@ -1178,9 +1218,9 @@ crunch typ_at [wp]: unmap_page "\<lambda>s. P (typ_at T p s)"
 lemmas unmap_page_typ_ats [wp] = abs_typ_at_lifts [OF unmap_page_typ_at]
 
 lemma pt_lookup_slot_cap_to:
-  "\<lbrakk> invs s; \<exists>\<rhd>(max_pt_level, pt) s; is_aligned pt pt_bits; vptr \<in> user_region;
+  "\<lbrakk> invs s; \<exists>\<rhd>(max_pt_level, pt) s; is_aligned pt (pt_bits FIXME_level); vptr \<in> user_region;
      pt_lookup_slot pt vptr (ptes_of s) = Some (level, slot) \<rbrakk>
-   \<Longrightarrow> \<exists>p cap. caps_of_state s p = Some cap \<and> is_pt_cap cap \<and> obj_refs cap = {table_base slot} \<and>
+   \<Longrightarrow> \<exists>p cap. caps_of_state s p = Some cap \<and> is_pt_cap cap \<and> obj_refs cap = {table_base FIXME_level slot} \<and>
                s \<turnstile> cap \<and> cap_asid cap \<noteq> None"
   apply (clarsimp simp: pt_lookup_slot_def pt_lookup_slot_from_level_def)
   apply (frule pt_walk_max_level)
@@ -1196,40 +1236,45 @@ lemma pt_lookup_slot_cap_to:
    apply (fastforce intro: valid_objs_caps)
   apply (frule pts_of_Some_alignedD, fastforce)
   apply (frule caps_of_state_valid, fastforce)
+  sorry (* FIXME AARCH64
   apply (fastforce simp: cap_asid_def is_cap_simps)
-  done
+  done *)
 
 lemma find_vspace_for_asid_cap_to:
   "\<lbrace>invs\<rbrace>
    find_vspace_for_asid asid
    \<lbrace>\<lambda>rv s.  \<exists>a b cap. caps_of_state s (a, b) = Some cap \<and> obj_refs cap = {rv} \<and>
-                      is_pt_cap cap \<and> s \<turnstile> cap \<and> is_aligned rv pt_bits\<rbrace>, -"
+                      is_pt_cap cap \<and> s \<turnstile> cap \<and> is_aligned rv (pt_bits pt_t)\<rbrace>, -"
   apply wpsimp
   apply (drule vspace_for_asid_vs_lookup)
   apply (frule valid_vspace_objs_strongD[rotated]; clarsimp)
   apply (frule pts_of_Some_alignedD, fastforce)
+  sorry (* FIXME AARCH64
   apply simp
   apply (drule vs_lookup_table_target, simp)
   apply (drule valid_vs_lookupD; clarsimp simp: vref_for_level_def)
   apply (frule (1) cap_to_pt_is_pt_cap, simp)
    apply (fastforce intro: valid_objs_caps)
   apply (fastforce intro: caps_of_state_valid cap_to_pt_is_pt_cap)
-  done
+  done *)
 
 lemma ex_pt_cap_eq:
   "(\<exists>ref cap. caps_of_state s ref = Some cap \<and> obj_refs cap = {p} \<and> is_pt_cap cap) =
-   (\<exists>ref asid. caps_of_state s ref = Some (ArchObjectCap (PageTableCap p asid)))"
-  by (fastforce simp add: is_pt_cap_def obj_refs_def is_PageTableCap_def)
+   (\<exists>ref asid. caps_of_state s ref = Some (ArchObjectCap (PageTableCap p pt_t asid)))"
+  sorry (* FIXME AARCH64
+  by (fastforce simp add: is_pt_cap_def obj_refs_def is_PageTableCap_def) *)
 
 lemma pt_bits_left_not_asid_pool_size:
   "pt_bits_left asid_pool_level \<noteq> pageBitsForSize sz"
-  by (cases sz; simp add: pt_bits_left_def bit_simps asid_pool_level_size)
+  sorry (* FIXME AARCH64
+  by (cases sz; simp add: pt_bits_left_def bit_simps asid_pool_level_size) *)
 
 lemma unmap_page_invs:
   "\<lbrace>invs and K (vptr \<in> user_region \<and> vmsz_aligned vptr sz)\<rbrace>
    unmap_page sz asid vptr pptr
    \<lbrace>\<lambda>_. invs\<rbrace>"
   unfolding unmap_page_def
+  sorry (* FIXME AARCH64
   apply (wpsimp wp: store_pte_invs_unmap)
   apply (rule conjI; clarsimp)
   apply (frule (1) pt_lookup_slot_vs_lookup_slotI)
@@ -1248,7 +1293,7 @@ lemma unmap_page_invs:
   apply clarsimp
   apply (drule (3) vs_lookup_table_vspace)
   apply (simp add: table_index_max_level_slots)
-  done
+  done *)
 
 lemma set_mi_invs[wp]: "\<lbrace>invs\<rbrace> set_message_info t a \<lbrace>\<lambda>x. invs\<rbrace>"
   by (simp add: set_message_info_def, wp)
@@ -1256,7 +1301,7 @@ lemma set_mi_invs[wp]: "\<lbrace>invs\<rbrace> set_message_info t a \<lbrace>\<l
 lemma data_at_orth:
   "data_at a p s
    \<Longrightarrow> \<not> ep_at p s \<and> \<not> ntfn_at p s \<and> \<not> cap_table_at sz p s \<and> \<not> tcb_at p s \<and> \<not> asid_pool_at p s
-         \<and> \<not> pt_at p s \<and> \<not> asid_pool_at p s"
+         \<and> \<not> pt_at pt_t p s \<and> \<not> asid_pool_at p s"
   apply (clarsimp simp: data_at_def obj_at_def a_type_def)
   apply (case_tac "kheap s p",simp)
   subgoal for ko by (case_tac ko,auto simp add: is_ep_def is_ntfn_def is_cap_table_def is_tcb_def)
@@ -1264,8 +1309,9 @@ lemma data_at_orth:
 
 lemma data_at_frame_cap:
   "\<lbrakk>data_at sz p s; valid_cap cap s; p \<in> obj_refs cap\<rbrakk> \<Longrightarrow> is_frame_cap cap"
+  sorry (* FIXME AARCH64
   by (cases cap; clarsimp simp: is_frame_cap_def valid_cap_def valid_arch_cap_ref_def data_at_orth
-                         split: option.splits arch_cap.splits)
+                         split: option.splits arch_cap.splits) *)
 
 lemma perform_pg_inv_get_addr[wp]:
   "\<lbrace>invs and valid_page_inv (PageGetAddr ptr)\<rbrace> perform_pg_inv_get_addr ptr \<lbrace>\<lambda>_. invs\<rbrace>"
@@ -1273,13 +1319,15 @@ lemma perform_pg_inv_get_addr[wp]:
 
 lemma unmap_page_pool_for_asid[wp]:
   "unmap_page pgsz asid vref pt \<lbrace>\<lambda>s. P (pool_for_asid asid s)\<rbrace>"
-  unfolding unmap_page_def by (wpsimp simp: pool_for_asid_def)
+  sorry (* FIXME AARCH64
+  unfolding unmap_page_def by (wpsimp simp: pool_for_asid_def) *)
 
 lemma data_at_level:
   "\<lbrakk> data_at pgsz p s; data_at (vmpage_size_of_level level) p s;
      pt_bits_left level' = pageBitsForSize pgsz; level \<le> max_pt_level \<rbrakk> \<Longrightarrow>
    level = level'"
-  by (fastforce simp: data_at_def obj_at_def)
+  sorry (* FIXME AARCH64
+  by (fastforce simp: data_at_def obj_at_def) *)
 
 lemma pt_lookup_slot_vs_lookup_slotI0:
   "\<lbrakk> vspace_for_asid asid s = Some pt_ptr;
@@ -1305,6 +1353,7 @@ lemma unmap_page_not_target:
          vs_lookup_slot_pool_for_asid[simp]
          pool_for_asid_vs_lookup[simp]
   apply (wpsimp wp: store_pte_invalid_vs_lookup_target_unmap)
+  sorry (* FIXME AARCH64
   apply (rule conjI; clarsimp)
    apply (clarsimp simp: vs_lookup_target_def vspace_for_asid_def obind_def vs_lookup_slot_def
                          vs_lookup_table_def
@@ -1363,11 +1412,12 @@ lemma unmap_page_not_target:
   apply clarsimp
   apply (subst (asm) pt_walk.simps)
   apply clarsimp
-  done
+  done *)
 
 lemma perform_pg_inv_unmap[wp]:
   "\<lbrace>invs and valid_page_inv (PageUnmap cap ct_slot)\<rbrace> perform_pg_inv_unmap cap ct_slot \<lbrace>\<lambda>_. invs\<rbrace>"
   unfolding perform_pg_inv_unmap_def
+  sorry (* FIXME AARCH64
   apply (wpsimp wp: arch_update_cap_invs_unmap_page hoare_vcg_ex_lift hoare_vcg_ball_lift
                     hoare_vcg_all_lift hoare_vcg_const_imp_lift get_cap_wp unmap_page_cte_wp_at
                     hoare_vcg_imp_lift'
@@ -1380,13 +1430,14 @@ lemma perform_pg_inv_unmap[wp]:
   apply (clarsimp simp: valid_unmap_def cap_master_cap_simps valid_cap_def wellformed_mapdata_def
                         cap_aligned_def)
   apply (fastforce simp: data_at_def split: if_split_asm intro: valid_objs_caps)
-  done
+  done *)
 
 lemma perform_pg_inv_map_invs[wp]:
-  "\<lbrace>invs and valid_page_inv (PageMap cap ct_slot (pte, slot))\<rbrace>
-   perform_pg_inv_map cap ct_slot pte slot
+  "\<lbrace>invs and valid_page_inv (PageMap cap ct_slot (pte, slot, level))\<rbrace>
+   perform_pg_inv_map cap ct_slot pte slot level
    \<lbrace>\<lambda>_. invs\<rbrace>"
   unfolding perform_pg_inv_map_def
+  sorry (* FIXME AARCH64
   apply (wpsimp wp: store_pte_invs arch_update_cap_invs_map hoare_vcg_all_lift hoare_vcg_imp_lift')
   apply (clarsimp simp: valid_page_inv_def cte_wp_at_caps_of_state is_arch_update_def is_cap_simps
                         cap_master_cap_simps parent_for_refs_def valid_slots_def same_ref_def)
@@ -1428,12 +1479,13 @@ lemma perform_pg_inv_map_invs[wp]:
   apply (drule (1) pt_slot_offset_vref_for_level; simp)
   apply (cases ct_slot)
   apply fastforce
-  done
+  done *)
 
 lemma perform_page_invs [wp]:
   "\<lbrace>invs and valid_page_inv pg_inv\<rbrace> perform_page_invocation pg_inv \<lbrace>\<lambda>_. invs\<rbrace>"
   unfolding perform_page_invocation_def
-  by (cases pg_inv; wpsimp)
+  sorry (* FIXME AARCH64
+  by (cases pg_inv; wpsimp) *)
 
 lemma asid_high_low:
   "\<lbrakk> asid_high_bits_of asid = asid_high_bits_of asid';
@@ -1442,6 +1494,7 @@ lemma asid_high_low:
   unfolding asid_high_bits_of_def asid_low_bits_of_def asid_high_bits_def asid_low_bits_def
   by word_bitwise simp
 
+typ asid_pool_entry
 end
 
 locale asid_pool_map = Arch +
@@ -1449,12 +1502,12 @@ locale asid_pool_map = Arch +
   defines "s' \<equiv> s\<lparr>kheap := kheap s(ap \<mapsto> ArchObj (ASIDPool (pool(asid_low_bits_of asid \<mapsto> ptp))))\<rparr>"
   assumes ap:  "asid_pools_of s ap = Some pool"
   assumes new: "pool (asid_low_bits_of asid) = None"
-  assumes pt:  "pts_of s ptp = Some pt"
-  assumes empty: "kernel_mappings_only pt s"
+  assumes pt:  "pts_of s (ap_vspace ptp) = Some pt"
+  (* FIXME AARCH64 assumes empty: "kernel_mappings_only pt s" *)
   assumes lookup: "pool_for_asid asid s = Some ap"
   assumes valid_vspace_objs: "valid_vspace_objs s"
   assumes valid_asids: "valid_asid_table s"
-  assumes aligned: "is_aligned ptp pt_bits"
+  assumes aligned: "\<And>pt_t. is_aligned (ap_vspace ptp) (pt_bits pt_t)" (*FIXME AARCH64: no idea *)
 begin
 
 lemma arch_state[simp]:
@@ -1479,15 +1532,16 @@ qed
 
 lemma empty_for_user:
   "vref \<in> user_region \<Longrightarrow>
-   pt (table_index (pt_slot_offset max_pt_level ptp vref)) = InvalidPTE"
+   pt_apply pt (table_index pt_t (pt_slot_offset max_pt_level (ap_vspace ptp) vref)) = InvalidPTE"
+  sorry (* FIXME AARCH64
   using empty aligned
-  by (clarsimp simp: kernel_mappings_only_def table_index_max_level_slots)
+  by (clarsimp simp: kernel_mappings_only_def table_index_max_level_slots) *)
 
 lemma vs_lookup_table:
   "vref \<in> user_region \<Longrightarrow>
    vs_lookup_table level asid' vref s' =
      (if asid' = asid \<and> level \<le> max_pt_level
-      then Some (max_pt_level, ptp)
+      then Some (max_pt_level, (ap_vspace ptp))
       else vs_lookup_table level asid' vref s)"
   apply clarsimp
   apply (rule conjI; clarsimp)
@@ -1498,6 +1552,7 @@ lemma vs_lookup_table:
    using pt aligned
    apply (clarsimp simp: obind_def ptes_of_def empty_for_user)
    apply (simp add: pt_slot_offset_def)
+  sorry (* FIXME AARCH64
    apply (erule notE)
    apply (rule is_aligned_add)
     apply (erule is_aligned_weaken)
@@ -1519,13 +1574,13 @@ lemma vs_lookup_table:
    apply (drule (1) asid_high_low)
    apply clarsimp
   apply (clarsimp simp: vspace_for_pool_def split: if_split_asm)
-  done
+  done *)
 
 lemma vs_lookup_slot:
   "vref \<in> user_region \<Longrightarrow>
    vs_lookup_slot level asid' vref s' =
      (if asid' = asid \<and> level \<le> max_pt_level
-      then Some (max_pt_level, pt_slot_offset max_pt_level ptp vref)
+      then Some (max_pt_level, pt_slot_offset max_pt_level (ap_vspace ptp) vref)
       else vs_lookup_slot level asid' vref s)"
   apply (simp add: vs_lookup_slot_def)
   apply (rule conjI; clarsimp)
@@ -1534,25 +1589,28 @@ lemma vs_lookup_slot:
   done
 
 lemma pte_refs_of_None:
-  "vref \<in> user_region \<Longrightarrow> pte_refs_of s (pt_slot_offset max_pt_level ptp vref) = None"
+  "vref \<in> user_region \<Longrightarrow> pte_refs_of pt_t (pt_slot_offset max_pt_level (ap_vspace ptp) vref) s = None"
   using aligned pt
-  by (clarsimp simp: ptes_of_def obind_def opt_map_def empty_for_user split: option.splits)
+  sorry (* FIXME AARCH64
+  by (clarsimp simp: ptes_of_def obind_def opt_map_def empty_for_user split: option.splits) *)
 
 lemma vs_lookup_table_None:
   "level \<le> max_pt_level \<Longrightarrow> vs_lookup_table level asid vref s = None"
   using lookup new ap
+  sorry (* FIXME AARCH64
   by (clarsimp simp: vs_lookup_table_def obind_def pool_for_asid_def vspace_for_pool_def
-               split: option.splits)
+               split: option.splits) *)
 
 lemma vs_lookup_slot_None:
   "level \<le> max_pt_level \<Longrightarrow> vs_lookup_slot level asid vref s = None"
-  by (clarsimp simp: vs_lookup_slot_def obind_def vs_lookup_table_None)
+  sorry (* FIXME AARCH64
+  by (clarsimp simp: vs_lookup_slot_def obind_def vs_lookup_table_None) *)
 
 lemma vs_lookup_target:
   "vref \<in> user_region \<Longrightarrow>
    vs_lookup_target level asid' vref s' =
      (if asid' = asid \<and> level = asid_pool_level
-      then Some (level, ptp)
+      then Some (level, ap_vspace ptp)
       else vs_lookup_target level asid' vref s)"
   apply clarsimp
   apply (rule conjI; clarsimp)
@@ -1562,6 +1620,7 @@ lemma vs_lookup_target:
    apply (simp add: pool_for_asid_def vspace_for_pool_def in_omonad)
   apply (cases "asid' = asid")
    apply clarsimp
+  sorry (* FIXME AARCH64
    apply (clarsimp simp: vs_lookup_target_def)
    apply (clarsimp simp: obind_def vs_lookup_slot_None vs_lookup_slot pte_refs_of_None)
   apply clarsimp
@@ -1584,7 +1643,7 @@ lemma vs_lookup_target:
   apply (drule (2) inj_on_domD[rotated])
   apply (drule (1) asid_high_low)
   apply clarsimp
-  done
+  done *)
 
 lemma valid_pool:
   "valid_vspace_obj asid_pool_level (ASIDPool pool) s"
@@ -1609,7 +1668,7 @@ lemma valid_vspace_obj:
 
 end
 
-context Arch begin global_naming RISCV64
+context Arch begin global_naming AARCH64
 
 lemma set_asid_pool_arch_objs_map:
   "\<lbrace>valid_vspace_objs and valid_arch_state and valid_global_objs and
@@ -1617,12 +1676,13 @@ lemma set_asid_pool_arch_objs_map:
     (\<lambda>s. asid_pools_of s ap = Some pool) and
     K (pool (asid_low_bits_of asid) = None) and
     (\<lambda>s. pool_for_asid asid s = Some ap) and
-    (\<lambda>s. \<exists>pt. pts_of s pt_ptr = Some pt \<and> kernel_mappings_only pt s) \<rbrace>
-  set_asid_pool ap (pool(asid_low_bits_of asid \<mapsto> pt_ptr))
+    (\<lambda>s. \<exists>pt. pts_of s (ap_vspace ape) = Some pt \<and> kernel_mappings_only pt s) \<rbrace>
+  set_asid_pool ap (pool(asid_low_bits_of asid \<mapsto> ape))
   \<lbrace>\<lambda>rv. valid_vspace_objs\<rbrace>"
   unfolding set_asid_pool_def
   supply fun_upd_apply[simp del]
   apply (wpsimp wp: set_object_wp)
+  sorry (* FIXME AARCH64
   apply (frule (5) asid_pool_map.intro)
     apply (clarsimp simp: valid_arch_state_def)
    apply (erule pspace_aligned_pts_ofD, simp)
@@ -1638,7 +1698,7 @@ lemma set_asid_pool_arch_objs_map:
   apply (rule conjI; clarsimp)
   apply (frule asid_pool_map.valid_pool)
   apply (fastforce simp: obj_at_def)
-  done
+  done *)
 
 lemma caps_of_state_fun_upd:
   "obj_at (same_caps val) p s \<Longrightarrow>
@@ -1653,13 +1713,14 @@ lemma set_asid_pool_valid_arch_caps_map:
     (\<lambda>s. asid_pools_of s ap = Some pool \<and> pool_for_asid asid s = Some ap \<and>
          (\<exists>ptr cap. caps_of_state s ptr = Some cap \<and> obj_refs cap = {pt_ptr} \<and>
                     vs_cap_ref cap = Some (asid, 0)))
-    and (\<lambda>s. \<exists>pt. pts_of s pt_ptr = Some pt \<and> kernel_mappings_only pt s)
+    and (\<lambda>s. \<exists>pt. pts_of s (ap_vspace ape) = Some pt \<and> kernel_mappings_only pt s)
     and K (pool (asid_low_bits_of asid) = None \<and> 0 < asid)\<rbrace>
-  set_asid_pool ap (pool(asid_low_bits_of asid \<mapsto> pt_ptr))
+  set_asid_pool ap (pool(asid_low_bits_of asid \<mapsto> ape))
   \<lbrace>\<lambda>rv. valid_arch_caps\<rbrace>"
   unfolding set_asid_pool_def
   supply fun_upd_apply[simp del]
   apply (wpsimp wp: set_object_wp)
+  sorry (* FIXME AARCH64
   apply (frule (5) asid_pool_map.intro)
     apply (clarsimp simp: valid_arch_state_def)
    apply (erule pspace_aligned_pts_ofD, simp)
@@ -1671,12 +1732,14 @@ lemma set_asid_pool_valid_arch_caps_map:
   apply simp
   apply (clarsimp simp: valid_vs_lookup_def caps_of_state_fun_upd obj_at_def)
   apply (clarsimp simp: asid_pool_map.vs_lookup_target split: if_split_asm)
-  by (fastforce simp: vref_for_level_asid_pool user_region_def)
+  by (fastforce simp: vref_for_level_asid_pool user_region_def) *)
 
+(* FIXME AARCH64
 lemma kernel_mappings_only_has:
   "kernel_mappings_only pt s \<Longrightarrow> has_kernel_mappings pt s"
-  by (simp add: kernel_mappings_only_def)
+  by (simp add: kernel_mappings_only_def) *)
 
+(* FIXME AARCH64
 lemma toplevel_pt_has_kernel_mappings:
   assumes ap: "pool_for_asid asid s = Some ap"
   assumes pool: "asid_pools_of s ap = Some pool"
@@ -1701,29 +1764,31 @@ proof -
                        vs_lookup_table_def vspace_for_asid_def word_neq_0_conv)
   with km pt
   show ?thesis by (simp add: equal_kernel_mappings_def)
-qed
+qed *)
 
 lemma set_asid_pool_invs_map:
   "\<lbrace>invs and
     (\<lambda>s. asid_pools_of s ap = Some pool \<and> pool_for_asid asid s = Some ap \<and>
          (\<exists>ptr cap. caps_of_state s ptr = Some cap \<and> obj_refs cap = {pt_ptr} \<and>
                     vs_cap_ref cap = Some (asid, 0)))
-    and (\<lambda>s. \<exists>pt. pts_of s pt_ptr = Some pt \<and> kernel_mappings_only pt s)
+    and (\<lambda>s. \<exists>pt. pts_of s (ap_vspace ape) = Some pt \<and> kernel_mappings_only pt s)
     and K (pool (asid_low_bits_of asid) = None \<and> 0 < asid)\<rbrace>
-  set_asid_pool ap (pool(asid_low_bits_of asid \<mapsto> pt_ptr))
+  set_asid_pool ap (pool(asid_low_bits_of asid \<mapsto> ape))
   \<lbrace>\<lambda>rv. invs\<rbrace>"
   apply (simp add: invs_def valid_state_def valid_pspace_def valid_asid_map_def)
+  sorry (* FIXME AARCH64
   apply (wpsimp wp: valid_irq_node_typ set_asid_pool_typ_at set_asid_pool_arch_objs_map
                     valid_irq_handlers_lift set_asid_pool_valid_arch_caps_map)
   apply (erule disjE, clarsimp simp: kernel_mappings_only_has)
   apply (erule (4) toplevel_pt_has_kernel_mappings)
   apply (simp add: valid_arch_caps_def)
-  done
+  done *)
 
 lemma ako_asid_pools_of:
   "ako_at (ASIDPool pool) ap s = (asid_pools_of s ap = Some pool)"
   by (clarsimp simp: obj_at_def in_omonad)
 
+(* FIXME AARCH64
 lemma copy_global_mappings_asid_pools[wp]:
   "copy_global_mappings pt_ptr \<lbrace>\<lambda>s. P (asid_pools_of s)\<rbrace>"
   unfolding copy_global_mappings_def by (wpsimp wp: mapM_x_wp')
@@ -1735,13 +1800,14 @@ lemma copy_global_mappings_pool_for_asid[wp]:
 lemma copy_global_mappings_caps_of_state[wp]:
   "copy_global_mappings pt_ptr \<lbrace>\<lambda>s. P (caps_of_state s)\<rbrace>"
   unfolding copy_global_mappings_def by (wpsimp wp: mapM_x_wp')
+*)
 
 lemma store_pte_vs_lookup_target_unreachable:
-  "\<lbrace>\<lambda>s. (\<forall>level. \<not> \<exists>\<rhd> (level, table_base p) s) \<and>
+  "\<lbrace>\<lambda>s. (\<forall>level. \<not> \<exists>\<rhd> (level, table_base pt_t p) s) \<and>
         vref \<in> user_region \<and>
         vs_lookup_target bot_level asid vref s \<noteq> Some (level, p') \<and>
         pspace_aligned s \<and> valid_vspace_objs s \<and> valid_asid_table s \<rbrace>
-   store_pte p pte
+   store_pte pt_t p pte
    \<lbrace>\<lambda>rv s. vs_lookup_target bot_level asid vref s \<noteq> Some (level, p')\<rbrace>"
   unfolding store_pte_def set_pt_def
   apply (wpsimp wp: set_object_wp)
@@ -1749,11 +1815,11 @@ lemma store_pte_vs_lookup_target_unreachable:
   done
 
 lemma store_pte_vs_lookup_table_unreachable:
-  "\<lbrace>\<lambda>s. (\<forall>level. \<not> \<exists>\<rhd> (level, table_base p) s) \<and>
+  "\<lbrace>\<lambda>s. (\<forall>level. \<not> \<exists>\<rhd> (level, table_base pt_t p) s) \<and>
         vref \<in> user_region \<and>
         vs_lookup_table bot_level asid vref s \<noteq> Some (level, p') \<and>
         pspace_aligned s \<and> valid_vspace_objs s \<and> valid_asid_table s \<rbrace>
-   store_pte p pte
+   store_pte pt_t p pte
    \<lbrace>\<lambda>rv s. vs_lookup_table bot_level asid vref s \<noteq> Some (level, p')\<rbrace>"
   unfolding store_pte_def set_pt_def
   apply (wpsimp wp: set_object_wp)
@@ -1761,15 +1827,16 @@ lemma store_pte_vs_lookup_table_unreachable:
   done
 
 lemma store_pte_valid_arch_state_unreachable:
-  "\<lbrace>valid_arch_state and valid_global_vspace_mappings and (\<lambda>s. table_base p \<notin> global_refs s) \<rbrace>
-   store_pte p pte
+  "\<lbrace>valid_arch_state and valid_global_vspace_mappings and (\<lambda>s. table_base pt_t p \<notin> global_refs s) \<rbrace>
+   store_pte pt_t p pte
    \<lbrace>\<lambda>_. valid_arch_state\<rbrace>"
-  unfolding valid_arch_state_def by (wpsimp wp: store_pte_valid_global_tables)
+  sorry (* FIXME AARCH64
+  unfolding valid_arch_state_def by (wpsimp wp: store_pte_valid_global_tables) *)
 
 lemma store_pte_valid_vs_lookup_unreachable:
   "\<lbrace>valid_vs_lookup and pspace_aligned and valid_vspace_objs and valid_asid_table and
-    (\<lambda>s. \<forall>level. \<not> \<exists>\<rhd> (level, table_base p) s)\<rbrace>
-   store_pte p pte
+    (\<lambda>s. \<forall>level. \<not> \<exists>\<rhd> (level, table_base pt_t p) s)\<rbrace>
+   store_pte pt_t p pte
    \<lbrace>\<lambda>_. valid_vs_lookup\<rbrace>"
   unfolding valid_vs_lookup_def
   apply (wpsimp wp: hoare_vcg_all_lift hoare_vcg_imp_lift' store_pte_vs_lookup_target_unreachable)
@@ -1778,25 +1845,27 @@ lemma store_pte_valid_vs_lookup_unreachable:
 
 lemma store_pte_valid_arch_caps_unreachable:
   "\<lbrace> invs and
-     (\<lambda>s. \<forall>level. \<not> \<exists>\<rhd> (level, table_base p) s) and
-     (\<lambda>s. \<forall>slot asidopt. caps_of_state s slot = Some (ArchObjectCap (PageTableCap (table_base p) asidopt))
+     (\<lambda>s. \<forall>level. \<not> \<exists>\<rhd> (level, table_base pt_t p) s) and
+     (\<lambda>s. \<forall>slot asidopt. caps_of_state s slot = Some (ArchObjectCap (PageTableCap (table_base pt_t p) pt_t asidopt))
                           \<longrightarrow> asidopt \<noteq> None) and
-     (\<lambda>s. table_base p \<notin> global_refs s) \<rbrace>
-   store_pte p pte
+     (\<lambda>s. table_base pt_t p \<notin> global_refs s) \<rbrace>
+   store_pte pt_t p pte
    \<lbrace> \<lambda>_. valid_arch_caps \<rbrace>"
   unfolding valid_arch_caps_def
+  sorry (* FIXME AARCH64
   apply (wpsimp wp: store_pte_valid_vs_lookup_unreachable store_pte_valid_table_caps)
-  by (fastforce simp: invs_def valid_state_def valid_arch_caps_def intro: valid_objs_caps)
+  by (fastforce simp: invs_def valid_state_def valid_arch_caps_def intro: valid_objs_caps) *)
 
 lemma store_pte_invs_unreachable:
   "\<lbrace>invs and
-    (\<lambda>s. \<forall>level. \<not> \<exists>\<rhd> (level, table_base p) s) and
+    (\<lambda>s. \<forall>level. \<not> \<exists>\<rhd> (level, table_base pt_t p) s) and
     K (wellformed_pte pte) and
-    (\<lambda>s. \<forall>slot asidopt. caps_of_state s slot = Some (ArchObjectCap (PageTableCap (table_base p) asidopt))
+    (\<lambda>s. \<forall>slot asidopt. caps_of_state s slot = Some (ArchObjectCap (PageTableCap (table_base pt_t p) pt_t asidopt))
                          \<longrightarrow> asidopt \<noteq> None) and
-    (\<lambda>s. table_base p \<notin> global_refs s) \<rbrace>
-  store_pte p pte \<lbrace>\<lambda>_. invs\<rbrace>"
+    (\<lambda>s. table_base pt_t p \<notin> global_refs s) \<rbrace>
+  store_pte pt_t p pte \<lbrace>\<lambda>_. invs\<rbrace>"
   unfolding invs_def valid_state_def valid_pspace_def
+  sorry (* FIXME AARCH64
   apply (wpsimp wp: store_pte_valid_arch_state_unreachable store_pte_valid_arch_caps_unreachable
                     store_pte_equal_kernel_mappings_no_kernel_slots
                     store_pte_valid_global_vspace_mappings
@@ -1806,33 +1875,36 @@ lemma store_pte_invs_unreachable:
               cong: conj_cong)
   apply (rule conjI, fastforce dest!: vspace_for_asid_vs_lookup)
   apply (fastforce simp: valid_arch_state_def dest: riscv_global_pt_in_global_refs)
-  done
+  done *)
 
 lemma invs_valid_global_vspace_mappings[elim!]:
   "invs s \<Longrightarrow> valid_global_vspace_mappings s"
   by (clarsimp simp: invs_def valid_state_def)
 
 lemma is_aligned_pte_offset:
-  "is_aligned pt_ptr pt_bits \<Longrightarrow>
-   is_aligned (pt_ptr + (i << pte_bits)) pte_bits"
+  "is_aligned pt_ptr (pt_bits pt_t) \<Longrightarrow>
+   is_aligned (pt_ptr + (i << pte_bits)) (pte_bits)"
   apply (rule is_aligned_add)
    apply (erule is_aligned_weaken, simp add: bit_simps)
   apply (simp add: is_aligned_shiftl)
   done
 
 lemma ptes_of_from_pt:
-  "\<lbrakk> pts pt_ptr = Some pt; is_aligned pt_ptr pt_bits; i \<le> mask ptTranslationBits \<rbrakk> \<Longrightarrow>
+  "\<lbrakk> pts pt_ptr = Some pt; is_aligned pt_ptr (pt_bits pt_t); i \<le> mask (ptTranslationBits pt_t) \<rbrakk> \<Longrightarrow>
    pte_of (pt_ptr + (i << pte_bits)) pts = Some (pt (ucast i))"
-  by (clarsimp simp: ptes_of_def in_omonad table_base_plus table_index_plus is_aligned_pte_offset)
+  sorry (* FIXME AARCH64 check statement
+  by (clarsimp simp: ptes_of_def in_omonad table_base_plus table_index_plus is_aligned_pte_offset) *)
 
+(* FIXME AARCH64
 lemma ptes_of_from_pt_ucast:
   "\<lbrakk> pts_of s pt_ptr = Some pt; is_aligned pt_ptr pt_bits \<rbrakk> \<Longrightarrow>
    ptes_of s (pt_ptr + (ucast (i::pt_index) << pte_bits)) = Some (pt i)"
   apply (drule (1) ptes_of_from_pt[where i="ucast i"])
    apply (rule ucast_leq_mask, simp add: bit_simps)
   apply (simp add: is_down_def target_size_def source_size_def word_size ucast_down_ucast_id)
-  done
+  done *)
 
+(* FIXME AARCH64
 lemma copy_global_mappings_copies[wp]:
   "\<lbrace>invs and (\<lambda>s. pts_of s pt_ptr = Some empty_pt \<and> pt_ptr \<notin> global_refs s)\<rbrace>
    copy_global_mappings pt_ptr
@@ -1917,15 +1989,17 @@ lemma copy_global_mappings_invs:
      apply wp+
   apply clarsimp
   done
+*)
 
 lemma cap_asid_pt_None[simp]:
-  "(cap_asid (ArchObjectCap (PageTableCap p m)) = None) = (m = None)"
+  "(cap_asid (ArchObjectCap (PageTableCap p pt_t m)) = None) = (m = None)"
   by (simp add: cap_asid_def split: option.splits)
 
 lemma perform_asid_pool_invs [wp]:
   "\<lbrace>invs and valid_apinv api\<rbrace> perform_asid_pool_invocation api \<lbrace>\<lambda>_. invs\<rbrace>"
   apply (clarsimp simp: perform_asid_pool_invocation_def store_asid_pool_entry_def
                   split: asid_pool_invocation.splits)
+  sorry (* FIXME AARCH64
   apply (wpsimp wp: set_asid_pool_invs_map hoare_vcg_all_lift hoare_vcg_imp_lift'
                     copy_global_mappings_invs arch_update_cap_invs_map get_cap_wp set_cap_typ_at
                 simp: ako_asid_pools_of
@@ -1947,11 +2021,12 @@ lemma perform_asid_pool_invs [wp]:
   apply (rule conjI, clarsimp)
    apply (drule (1) unique_table_capsD[rotated]; clarsimp)
   apply fastforce
-  done
+  done *)
 
+(* FIXME AARCH64
 lemma invs_aligned_pdD:
   "\<lbrakk> pspace_aligned s; valid_arch_state s \<rbrakk> \<Longrightarrow> is_aligned (riscv_global_pt (arch_state s)) pt_bits"
-  by (clarsimp simp: valid_arch_state_def)
+  by (clarsimp simp: valid_arch_state_def) *)
 
 lemma do_machine_op_valid_kernel_mappings:
   "do_machine_op f \<lbrace>valid_kernel_mappings\<rbrace>"
@@ -1960,7 +2035,8 @@ lemma do_machine_op_valid_kernel_mappings:
 lemma valid_vspace_obj_default:
   assumes tyunt: "ty \<noteq> Structures_A.apiobject_type.Untyped"
   shows "ArchObj ao = default_object ty dev us \<Longrightarrow> valid_vspace_obj level ao s'"
-  by (cases ty; simp add: default_object_def tyunt)
+  sorry (* FIXME AARCH64
+  by (cases ty; simp add: default_object_def tyunt) *)
 
 end
 
