proof/invariant-abstract/AARCH64/ArchCSpaceInv_AI.thy
@@ -12,7 +12,7 @@ theory ArchCSpaceInv_AI
 imports CSpaceInv_AI
 begin
 
-context Arch begin global_naming RISCV64
+context Arch begin global_naming AARCH64
 
 definition
    safe_ioport_insert :: "cap \<Rightarrow> cap \<Rightarrow> 'a::state_ext state \<Rightarrow> bool"
@@ -120,11 +120,12 @@ lemma replace_cap_invs:
    apply (simp add: is_cap_simps)
   apply (elim disjE)
    apply simp
+   sorry (* FIXME AARCH64
    apply (clarsimp simp: valid_table_capsD[OF caps_of_state_cteD]
                     valid_arch_caps_def unique_table_refs_no_cap_asidE)
   apply (rule conjI, clarsimp)
   apply (rule conjI, rule Ball_emptyI, simp add: gen_obj_refs_subset)
-  by clarsimp
+  by clarsimp *)
 
 definition
   "is_simple_cap_arch cap \<equiv> \<not>is_pt_cap cap"
@@ -197,7 +198,7 @@ lemmas cap_asid_base_simps [simp] =
 definition
   "cap_vptr_arch acap \<equiv> case acap of
      (FrameCap _ _ _ _  (Some (_, vptr))) \<Rightarrow> Some vptr
-  |  (PageTableCap _ (Some (_, vptr))) \<Rightarrow> Some vptr
+  |  (PageTableCap _ _ (Some (_, vptr))) \<Rightarrow> Some vptr
   | _ \<Rightarrow> None"
 
 definition
