proof/invariant-abstract/AARCH64/ArchCSpace_AI.thy
@@ -12,7 +12,7 @@ theory ArchCSpace_AI
 imports CSpace_AI
 begin
 
-context Arch begin global_naming RISCV64
+context Arch begin global_naming AARCH64
 
 named_theorems CSpace_AI_assms
 
@@ -58,7 +58,8 @@ lemma weak_derived_valid_cap [CSpace_AI_assms]:
                     valid_cap_def cap_aligned_def bits_of_def
                     aobj_ref_cases Let_def cap_asid_def
              split: cap.splits arch_cap.splits option.splits)
-  done
+  sorry (* FIXME AARCH64
+  done *)
 
 lemma copy_obj_refs [CSpace_AI_assms]:
   "copy_of cap cap' \<Longrightarrow> obj_refs cap' = obj_refs cap"
@@ -138,11 +139,12 @@ lemma set_untyped_cap_as_full_valid_arch_caps [CSpace_AI_assms]:
    \<lbrace>\<lambda>ya. valid_arch_caps\<rbrace>"
   supply if_split[split del]
   apply (clarsimp simp: valid_arch_caps_def set_untyped_cap_as_full_def)
+  sorry (* FIXME AARCH64
   apply (wpsimp wp: set_cap_valid_vs_lookup set_cap_valid_table_caps
                 simp_del: fun_upd_apply simp: cte_wp_at_caps_of_state)
   apply (fastforce simp: unique_table_refs_upd_eqD unique_table_caps_upd_eqD
                          is_cap_simps cte_wp_at_caps_of_state)
-  done
+  done *)
 
 lemma set_untyped_cap_as_full[wp, CSpace_AI_assms]:
   "\<lbrace>\<lambda>s. no_cap_to_obj_with_diff_ref a b s \<and> cte_wp_at ((=) src_cap) src s\<rbrace>
@@ -276,6 +278,7 @@ lemma cap_insert_valid_arch_caps [CSpace_AI_assms]:
       apply (erule_tac x=a in allE, erule_tac x=b in allE)
       apply simp+
     apply (clarsimp simp: obj_at_def is_cap_simps valid_arch_caps_def)
+    sorry (* FIXME AARCH64
     apply (frule(1) valid_table_capsD)
       apply (clarsimp simp: cte_wp_at_caps_of_state)
       apply (drule is_derived_is_pt)
@@ -296,7 +299,7 @@ lemma cap_insert_valid_arch_caps [CSpace_AI_assms]:
    apply (drule_tac ptr=src and ptr'="(x,xa)" in unique_table_capsD)
          apply (fastforce simp: cap_asid_def is_cap_simps)+
   apply (auto simp: cte_wp_at_caps_of_state)
-  done
+  done *)
 
 end
 
@@ -304,7 +307,7 @@ end
 global_interpretation cap_insert_crunches?: cap_insert_crunches .
 
 
-context Arch begin global_naming RISCV64
+context Arch begin global_naming AARCH64
 
 lemma cap_insert_cap_refs_in_kernel_window[wp, CSpace_AI_assms]:
   "\<lbrace>cap_refs_in_kernel_window
@@ -492,11 +495,12 @@ end
 global_interpretation CSpace_AI?: CSpace_AI
   proof goal_cases
   interpret Arch .
-  case 1 show ?case by (unfold_locales; (fact CSpace_AI_assms)?)
+  case 1 show ?case sorry (* FIXME AARCH64
+by (unfold_locales; (fact CSpace_AI_assms)?) *)
   qed
 
 
-context Arch begin global_naming RISCV64
+context Arch begin global_naming AARCH64
 
 lemma is_cap_simps':
   "is_cnode_cap cap = (\<exists>r bits g. cap = cap.CNodeCap r bits g)"
